src/new_goose_lang/lib/struct/impl.v
@@ -1,106 +1,17 @@
-From Perennial.goose_lang Require Import notation.
-From Perennial.new_goose_lang.lib Require Import typed_mem.impl.
+From Perennial.new_goose_lang.lib Require Import mem.impl.
 
-(** * Struct library
+Declare Scope struct_scope.
+Notation "f :: t" := (@pair string go_type f%string t) : struct_scope.
+Notation "f ::= v" := (@pair string val f%string v%V) (at level 60) : val_scope.
+Notation "f ::= v" := (@pair string expr f%string v%E) (at level 60) : expr_scope.
+Delimit Scope struct_scope with struct.
 
-    Access field offsets within pairs by name rather than using Fst and Snd. *)
-
-Set Default Proof Using "Type".
-Set Implicit Arguments.
-
+Module struct.
 Section goose_lang.
-Context `{ffi_sem: ffi_semantics}.
-
-Definition descriptor := list (string * go_type).
-Definition mkStruct (fs: list (string * go_type)): descriptor := fs.
-
-Class descriptor_wf (d:descriptor) : Set :=
-  { descriptor_NoDup: NoDup d.*1; }.
-
-Definition option_descriptor_wf (d:descriptor) : option (descriptor_wf d).
-  destruct (decide (NoDup d.*1)); [ apply Some | apply None ].
-  constructor; auto.
-Defined.
-
-Definition proj_descriptor_wf (d:descriptor) :=
-  match option_descriptor_wf d as mwf return match mwf with
-                                             | Some _ => descriptor_wf d
-                                             | None => True
-                                             end  with
-  | Some pf => pf
-  | None => I
-  end.
-
-Implicit Types (d:descriptor).
 Infix "=?" := (String.eqb).
 
-Fixpoint getField d (f0: string) : val :=
-  match d with
-  | [] => λ: <>, #()
-  | (f,_)::fs => if f =? f0
-               then (λ: "v", Fst (Var "v"))%V
-               else (λ: "v", getField fs f0 (Snd (Var "v")))%V
-  end.
-
-(* FIXME: what does _f mean? Want better name. *)
-Fixpoint getField_f d f0: val -> val :=
-  λ v, match d with
-       | [] => #()
-       | (f,_)::fs =>
-         match v with
-         | PairV v1 v2 => if f =? f0 then v1 else getField_f fs f0 v2
-         | _ => #()
-         end
-       end.
-
-Fixpoint setField_f d f0 fv: val -> val :=
-  λ v, match d with
-       | [] => v
-       | (f,_)::fs =>
-         match v with
-         | PairV v1 v2 =>
-           if f =? f0
-           then PairV fv v2
-           else PairV v1 (setField_f fs f0 fv v2)
-         | _ => v
-         end
-       end.
-
-Fixpoint assocl_lookup {A} (field_vals: list (string * A)) (f0: string) : option A :=
-  match field_vals with
-  | [] => None
-  | (f, v)::fs => if f =? f0 then Some v else assocl_lookup fs f0
-  end.
-
-Fixpoint build_struct_val d (field_vals: list (string*expr)): option expr :=
-  let lookup_f := assocl_lookup field_vals in
-  match d with
-  | [] => Some (Val #())
-  | (f,ft)::fs =>
-    let e := default (Val (zero_val ft)) (lookup_f f) in
-    match build_struct_val fs field_vals with
-    | Some e' => Some (e, e')%E
-    | None => None
-    end
-  end.
-
-Definition buildStruct d (fvs: list (string*expr)) : expr :=
-  match build_struct_val d fvs with
-  | Some v => v
-  | None => LitV LitUnit
-  end.
-
-Fixpoint buildStruct_f d (field_vals: list (string*val)): val :=
-  let lookup_f := assocl_lookup field_vals in
-  match d with
-  | [] => (#())
-  | (f,ft)::fs =>
-    let e := default (zero_val ft) (lookup_f f) in
-    let e' := buildStruct_f fs field_vals in
-    (e, e')%V
-  end.
-
-Fixpoint field_offset d f0 : (Z * go_type) :=
+Context `{ffi_syntax}.
+Fixpoint field_offset (d : struct.descriptor) f0 : (Z * go_type) :=
   match d with
   | [] => (-1, ptrT)
   | (f,t)::fs => if f =? f0 then (0, t)
@@ -109,50 +20,17 @@ Fixpoint field_offset d f0 : (Z * go_type) :=
                     end
   end.
 
-Definition fieldType (d:descriptor) (f:string): go_type :=
-  match field_offset d f with
-  | (_, t) => t
+
+Definition field_ref (d : struct.descriptor) f0: val :=
+  λ: "p", BinOp (OffsetOp (field_offset d f0).1) (Var "p") #1.
+
+Definition field_ty d f0 : go_type := (field_offset d f0).2.
+
+Fixpoint make (d : struct.descriptor) (field_vals: list (string*expr)) : expr :=
+  match d with
+  | [] => Val #()
+  | (f,ft)::fs => (default (Val (zero_val ft)) (assocl_lookup field_vals f), make fs field_vals)
   end.
 
-(** structFieldRef gives a function that takes a location and constant pointer
-arithmetic on it (which is pre-computed based on the field and descriptor). *)
-Definition structFieldRef d f0: val :=
-  λ: "p", BinOp (OffsetOp (field_offset d f0).1) (Var "p") #1
-.
-
-Definition structFieldRef_f d f0 l: loc :=
-  l +ₗ (field_offset d f0).1
-.
-
-Definition structFieldTy_f d f0 : go_type :=
-  (field_offset d f0).2
-.
-
 End goose_lang.
-
-#[global]
-Hint Extern 3 (descriptor_wf ?d) => exact (proj_descriptor_wf d) : typeclass_instances.
-
-Module struct.
-  Notation decl := mkStruct.
-  Notation wf := descriptor_wf.
-
-  Notation mk := buildStruct.
-  Notation mk_f := buildStruct_f.
-  Notation get := getField.
-  Notation fieldRef := structFieldRef.
-  Notation fieldRef_f := structFieldRef_f.
-
-  Notation fieldTy := structFieldTy_f.
 End struct.
-
-Declare Scope struct_scope.
-Notation "f :: t" := (@pair string go_type f%string t) : struct_scope.
-Notation "f ::= v" := (@pair string val f%string v%V) (at level 60) : val_scope.
-Notation "f ::= v" := (@pair string expr f%string v%E) (at level 60) : expr_scope.
-Delimit Scope struct_scope with struct.
-Arguments mkStruct _%struct_scope.
-
-(* TODO: we'll again need to unfold these to prove theorems about them, but
-for typechecking they should be opaque *)
-Global Opaque structFieldRef.
