src/new_goose_lang/lib/struct/struct.v
@@ -1,17 +1,74 @@
 From iris.proofmode Require Import coq_tactics reduction.
 From Perennial.base_logic.lib Require Import invariants.
 From Perennial.goose_lang Require Import proofmode.
-From Perennial.new_goose_lang.lib Require Export typed_mem struct.impl.
+From Perennial.new_goose_lang.lib Require Import mem typing.
+From Perennial.new_goose_lang.lib Require Export struct.impl.
 From Perennial.Helpers Require Import NamedProps.
 
-Notation "l ↦s[ d :: f ] dq v" := (struct.fieldRef_f d f l ↦[struct.fieldTy d f]{dq} v)%I
+Module struct.
+Section goose_lang.
+Context `{ffi_syntax}.
+
+Implicit Types (d : struct.descriptor).
+Infix "=?" := (String.eqb).
+(* FIXME: what does _f mean? Want better name. *)
+Fixpoint get_field_f d f0: val -> val :=
+  λ v, match d with
+       | [] => #()
+       | (f,_)::fs =>
+         match v with
+         | PairV v1 v2 => if f =? f0 then v1 else get_field_f fs f0 v2
+         | _ => #()
+         end
+       end.
+
+Fixpoint set_field_f d f0 fv: val -> val :=
+  λ v, match d with
+       | [] => v
+       | (f,_)::fs =>
+         match v with
+         | PairV v1 v2 =>
+           if f =? f0
+           then PairV fv v2
+           else PairV v1 (set_field_f fs f0 fv v2)
+         | _ => v
+         end
+       end.
+
+Definition field_ref_f d f0 l: loc := l +ₗ (struct.field_offset d f0).1.
+
+Class Wf (d : struct.descriptor) : Set :=
+  { descriptor_NoDup: NoDup d.*1; }.
+
+End goose_lang.
+End struct.
+
+Notation "l ↦s[ d :: f ] dq v" := (struct.field_ref_f d f l ↦[struct.field_ty d f]{dq} v)%I
   (at level 50, dq custom dfrac at level 70, d at level 59, f at level 59,
      format "l  ↦s[ d :: f ] dq  v").
 
+Definition option_descriptor_wf (d : struct.descriptor) : option (struct.Wf d).
+  destruct (decide (NoDup d.*1)); [ apply Some | apply None ].
+  constructor; auto.
+Defined.
+
+Definition proj_descriptor_wf (d : struct.descriptor) :=
+  match option_descriptor_wf d as mwf return match mwf with
+                                             | Some _ => struct.Wf d
+                                             | None => True
+                                             end  with
+  | Some pf => pf
+  | None => I
+  end.
+
+Global Hint Extern 3 (struct.Wf ?d) => exact (proj_descriptor_wf d) : typeclass_instances.
+
 Section lemmas.
+
 Context `{heapGS Σ}.
-(* FIXME: move this *)
-Local Fixpoint struct_big_fields_rec l dq (d: descriptor) (fs:descriptor) (v:val): iProp Σ :=
+
+Local Fixpoint struct_big_fields_rec l dq (d : struct.descriptor) (fs : struct.descriptor)
+      (v : val): iProp Σ :=
   match fs with
   | [] => "_" ∷ ⌜v = #()⌝
   | (f,t)::fs =>
@@ -24,9 +81,28 @@ Local Fixpoint struct_big_fields_rec l dq (d: descriptor) (fs:descriptor) (v:val
 
 Definition struct_fields l dq d v : iProp Σ := struct_big_fields_rec l dq d d v.
 
-Theorem struct_fields_split l q d {dwf: struct.wf d} v :
+Theorem struct_fields_split l q d {dwf: struct.Wf d} v :
   typed_pointsto l q (structT d) v ⊣⊢ struct_fields l q d v.
 Proof.
 Admitted.
 
 End lemmas.
+
+Section wps.
+Context `{sem: ffi_semantics} `{!ffi_interp ffi} `{!heapGS Σ}.
+
+Lemma wp_struct_fieldRef d f (l : loc) :
+  {{{ True }}}
+    (struct.field_ref d f) #l
+  {{{ RET #(struct.field_ref_f d f l); True }}}
+.
+Proof.
+  iIntros (?) "_ HΦ".
+  Transparent struct.field_ref. wp_lam. Opaque struct.field_ref.
+  wp_pures.
+  unfold struct.field_ref_f.
+  rewrite Z.mul_1_r.
+  by iApply "HΦ".
+Qed.
+
+End wps.
