src/new_goose_lang/lib/typing/typing.v
@@ -1,0 +1,149 @@
+From Perennial.new_goose_lang Require Import lib.typing.impl.
+
+(** * Typed data representations for struct and slice *)
+Module slice.
+Record t := mk { ptr: loc; sz: u64; cap: u64; }.
+Notation nil := slice_nil.
+
+Section goose_lang.
+  Context `{ffi_semantics}.
+  Definition val (s: slice.t) : val := (#s.(slice.ptr), #s.(slice.sz), #s.(slice.cap)).
+End goose_lang.
+End slice.
+
+Module struct.
+Section goose_lang.
+  Context `{ffi_syntax}.
+
+  Infix "=?" := (String.eqb).
+
+  Fixpoint val (d : struct.descriptor) (field_vals: list (string*val)): val :=
+    match d with
+    | [] => (#())
+    | (f,ft)::fs => (default (zero_val ft) (assocl_lookup field_vals f), val fs field_vals)
+    end.
+End goose_lang.
+End struct.
+
+Declare Scope struct_scope.
+Notation "f :: t" := (@pair string go_type f%string t) : struct_scope.
+Notation "f ::= v" := (@pair string val f%string v%V) (at level 60) : val_scope.
+Notation "f ::= v" := (@pair string expr f%string v%E) (at level 60) : expr_scope.
+Delimit Scope struct_scope with struct.
+
+(** * Pure Coq reasoning principles *)
+Section typing.
+  Context `{ffi_sem: ffi_semantics} `{!ffi_interp ffi}.
+
+  Program Definition go_type_ind :=
+    λ (P : go_type → Prop) (f : P boolT) (f0 : P uint8T) (f1 : P uint16T) (f2 : P uint32T)
+      (f3 : P uint64T) (f4 : P int8T) (f5 : P int16T) (f6 : P int32T) (f7 : P int64T)
+      (f8 : P stringT) (f9 : ∀ elem : go_type, P elem → P (sliceT elem))
+      (f10 : ∀ (decls : list (string * go_type)) (Hfields : ∀ t, In t decls.*2 → P t), P (structT decls))
+      (f11 : P ptrT) (f12 : P funcT) (f13 : P interfaceT)
+      (f14 : ∀ key : go_type, P key → ∀ elem : go_type, P elem → P (mapT key elem))
+      (f15 : ∀ elem : go_type, P elem → P (chanT elem)),
+    fix F (g : go_type) : P g :=
+      match g as g0 return (P g0) with
+      | boolT => f
+      | uint8T => f0
+      | uint16T => f1
+      | uint32T => f2
+      | uint64T => f3
+      | int8T => f4
+      | int16T => f5
+      | int32T => f6
+      | int64T => f7
+      | stringT => f8
+      | sliceT elem => f9 elem (F elem)
+      | structT decls => f10 decls _
+      | ptrT => f11
+      | funcT => f12
+      | interfaceT => f13
+      | mapT key elem => f14 key (F key) elem (F elem)
+      | chanT elem => f15 elem (F elem)
+      end.
+  Obligation 1.
+  intros.
+  revert H.
+  enough (Forall P decls.*2).
+  1:{
+    intros.
+    rewrite List.Forall_forall in H.
+    apply H. done.
+  }
+  induction decls; first done.
+  destruct a. apply Forall_cons. split.
+  { apply F. }
+  { apply IHdecls. }
+  Defined.
+
+  Inductive has_go_type : val → go_type → Prop :=
+  | has_go_type_bool (b : bool) : has_go_type #b boolT
+  | has_go_type_uint64 (x : w64) : has_go_type #x uint64T
+  | has_go_type_uint32 (x : w32) : has_go_type #x uint32T
+  | has_go_type_uint16 : has_go_type nil uint16T
+  | has_go_type_uint8 (x : w8) : has_go_type #x uint8T
+
+  | has_go_type_int64 (x : w64) : has_go_type #x int64T
+  | has_go_type_int32 (x : w32) : has_go_type #x int32T
+  | has_go_type_int16 : has_go_type nil int16T
+  | has_go_type_int8 (x : w8) : has_go_type #x int8T
+
+  | has_go_type_string (s : string) : has_go_type #(str s) stringT
+  | has_go_type_slice elem (s : slice.t) : has_go_type (slice.val s) (sliceT elem)
+  | has_go_type_slice_nil elem : has_go_type slice.nil (sliceT elem)
+
+  | has_go_type_struct
+      (d : struct.descriptor) fvs
+      (Hfields : ∀ f t, In (f, t) d → has_go_type (default (zero_val t) (assocl_lookup fvs f)) t)
+    : has_go_type (struct.val d fvs) (structT d)
+  | has_go_type_ptr (l : loc) : has_go_type #l ptrT
+  | has_go_type_func f e v : has_go_type (RecV f e v) funcT
+  | has_go_type_func_nil : has_go_type nil funcT
+
+  (* FIXME: interface_val *)
+  | has_go_type_interface (s : slice.t) : has_go_type (slice.val s) interfaceT
+  | has_go_type_interface_nil : has_go_type interface_nil interfaceT
+
+  | has_go_type_mapT kt vt (l : loc) : has_go_type #l (mapT kt vt)
+  | has_go_type_chanT t (l : loc) : has_go_type #l (chanT t)
+  .
+
+  Lemma zero_val_has_go_type t :
+    has_go_type (zero_val t) t.
+  Proof.
+    induction t using go_type_ind; try econstructor.
+    replace (zero_val (structT decls)) with (struct.val decls []).
+    {
+      econstructor. intros. simpl. apply Hfields.
+      apply in_map_iff. eexists _.
+      split; last done. done.
+    }
+    induction decls.
+    { simpl. replace (#()) with (struct.val [] []) by done. econstructor. }
+    destruct a. simpl.
+    f_equal.
+    apply IHdecls.
+    intros.
+    apply Hfields.
+    simpl. right. done.
+  Qed.
+
+  Lemma has_go_type_len {v t} :
+    has_go_type v t ->
+    length (flatten_struct v) = (go_type_size t).
+  Proof.
+    rewrite go_type_size_unseal.
+    induction 1; simpl; auto.
+    induction d.
+    { done. }
+    destruct a. cbn.
+    rewrite app_length.
+    rewrite IHd.
+    { f_equal. apply H. by left. }
+    { clear H IHd. intros. apply Hfields. by right. }
+    { intros. apply H. simpl. by right. }
+  Qed.
+
+End typing.
