src/new_goose_lang/prelude.v
@@ -1,10 +1,10 @@
 From Perennial.goose_lang Require Export lang notation.
-From Perennial.new_goose_lang Require Export exception loop.impl struct.impl typed_mem.impl.
+From Perennial.new_goose_lang Require Export exception typing.impl
+     loop.impl struct.impl mem.impl.
+(*
 From Perennial.goose_lang.lib Require Export
      encoding.impl map.impl slice.impl
      time.impl rand.impl string.impl channel.impl
-     noop.impl
-.
+     noop.impl. *)
 
-Open Scope heap_types.
 Open Scope struct_scope.
