src/program_proof/asyncfile/proof.v
@@ -120,7 +120,7 @@ Definition own_AsyncFile_internal f N γ P mu : iProp Σ :=
   ∃ data_sl fname (data:list u8) (idx durableIndex : u64) (indexCond durableIndexCond closedCond : loc)
     (closed closeRequested : bool) ,
   "#Hfilename" ∷ f ↦s[AsyncFile :: "filename"]□ #(str fname) ∗
-  "Hdata_sl" ∷ f ↦s[AsyncFile :: "data"] (slice_val data_sl) ∗
+  "Hdata_sl" ∷ f ↦s[AsyncFile :: "data"] (slice.val data_sl) ∗
   "#Hdata" ∷ own_slice_small data_sl byteT (DfracDiscarded) data ∗
   "Hindex" ∷ f ↦s[AsyncFile :: "index"] #idx ∗
   "HdurableIndex" ∷ f ↦s[AsyncFile :: "durableIndex"] #durableIndex ∗
